lock_t is not void* anymore, but a 24 or 40 bytes struct

progs/threads.h
@@ -1,20 +1,23 @@
-typedef void* lock_t;
-typedef void* cond_t;
+/* as far as I could determine, mutexes are 24 chars long on 32 bits,
+   40 chars long on 64 bit linux machines */
+/* typedef struct {char a[8]; void* b[4];} lock_t; */
+typedef struct lock_t {char a[8]; void* b[4];} lock_t;
 
-lock_t new_lock(void);
+void makelock(lock_t *lock);
 
-void make_lock(lock_t lock);
+void freelock(lock_t *lock);
 
-void free_lock(lock_t lock);
+void acquire(lock_t *lock);
 
-void acquire(lock_t lock);
-
-void release(lock_t lock);
+void release(lock_t *lock);
 
 void spawn_thread(void* (*f)(void*), void* args);
 
 void exit_thread(void);
 
-void wait(cond_t cv, lock_t lock);
+/* condition variables are 48 chars */
+typedef struct cond_t {char a[48];} cond_t;
 
-void signal(cond_t cv);
+void wait(cond_t *cv, lock_t *lock);
+
+void signal(cond_t *cv);
